

For the datasets of morphometric and clearance measurements, we simply calculated
means ($\bar{z}$) and standard errors ($s_{\bar{z}}$) for a species and 
intestinal position $p$ ($p \in \{ 1, 2, 3 \}$) as such:

\begin{equation}
\label{eq:aggr-sp-pos}
\begin{split}
    \mathbf{Z} &= 
\begin{bmatrix}
    f\left( x_{1,1} \right) & f\left( x_{1,2} \right) & f\left( x_{1,3} \right) \\
    f\left( x_{2,1} \right) & f\left( x_{2,2} \right) & f\left( x_{2,3} \right) \\
    \vdots & \vdots & \vdots \\
    f\left( x_{n,1} \right) & f\left( x_{n,2} \right) & f\left( x_{n,3} \right)
\end{bmatrix} \\
    \bar{z}_p &= \frac{1}{n} \sum_{i=1}^{n} \mathbf{Z}_{i,p} \\
    s_p &= \sqrt{ \frac{1}{n-1} \sum_{i=1}^{n}\left( \mathbf{Z}_{i,p} - \bar{z} \right)^2 } \\
    s_{\bar{z}(p)} &= \frac{ s_p }{ \sqrt{n} }
\end{split}
\end{equation}

where $f$ is the transformation function (either log or identity), 
$x_{i,p}$ is the $i$th untransformed value of the focal measurement for segment $p$,
and $n$ is the number of samples for the focal species.

For measurements that were aggregated by species but had separate measurements by
intestinal position, we did the following:

\begin{equation}
\label{eq:aggr-sp}
\begin{split}
    \mathbf{Z} &= 
\begin{bmatrix}
    f\left( x_{1,1} \right) & f\left( x_{1,2} \right) & f\left( x_{1,3} \right) \\
    f\left( x_{2,1} \right) & f\left( x_{2,2} \right) & f\left( x_{2,3} \right) \\
    \vdots & \vdots & \vdots \\
    f\left( x_{n,1} \right) & f\left( x_{n,2} \right) & f\left( x_{n,3} \right)
\end{bmatrix} \\[1ex]
    \mathbf{z} &= \frac{1}{3} \begin{bmatrix}
    \sum_{p=1}^{3} \mathbf{Z}_{1,p} \\[1ex]
    \sum_{p=1}^{3} \mathbf{Z}_{2,p} \\
    \vdots \\
    \sum_{p=1}^{3} \mathbf{Z}_{n,p}
\end{bmatrix} \\
    \bar{z} &= \frac{1}{n} \sum_{i=1}^{n} \mathbf{z}_{i} \\
    s_p &= \sqrt{ \frac{1}{n-1} \sum_{i=1}^{n}\left( \mathbf{z}_{i} - \bar{z} \right)^2 } \\
    s_{\bar{z}(p)} &= \frac{ s_p }{ \sqrt{n} }
\end{split}
\end{equation}


We could not do this for the fractional absorption data because different 
individuals were used for the various measurements necessary to get the final
parameter values for each species.
The final parameter, $a$, equals the following:

\begin{equation}
\label{eq:absorption}
    a = \frac{ e / b }{ t }
\end{equation}

where $b$ is probe content at the beginning,
$e$ is probe content at the end,
and $t$ is total intestinal surface area (i.e., $\text{NSA} \times \text{SEF}$).


For three species, the individuals used for measurements for this calculation are 
split into three groups:
One set of individuals were used for $b$, another for $e$, and a third
for $t$.
For the rest of the species, $b$ and $e$ were measured together, but
$t$ was measured in a different set of individuals.

This is important because 
$\mean{ \frac{X}{Y} } \ne \frac{ \mean{X} }{ \mean{Y} }$ and
$\var{ \frac{X}{Y} } \ne \frac{ \var{X} }{ \var{Y} }$.
But because $\mean{ X Y } = \mean{X} \mean{Y}$ and
$\var{XY} = \mean{X}^2 \var{Y} + \mean{Y}^2 \var{X} + \var{X} \var{Y}$,
we inversed estimates before taking means or variances to allow us to combine
these values.
(Since these are entirely different individuals, we're assuming they are 
independent samples.)

To begin, equation \ref{eq:absorption} can be manipulated to the following:

\begin{equation}
\label{eq:absorption2}
    a = e \left( \frac{1}{b} \right) \left( \frac{1}{ t } \right)
\end{equation}


Now we did the following to get mean absorptions ($\bar{a}$) for a given species:

\begin{equation}
\label{eq:absorption3}
\begin{split}
    \bar{e} &= \frac{1}{n_e}\sum_{i=1}^{n_e}\left( e_i \right) \\
    \bar{B} &= \frac{1}{n_b}\sum_{j=1}^{n_b}\left( \frac{1}{ b_j } \right) \\
    \bar{T} &= \frac{1}{n_t}\sum_{k=1}^{n_t}\left( \frac{1}{ t_k } \right) \\
    \bar{a} &= \bar{e} \bar{B} \bar{T}
\end{split}
\end{equation}

where $n_e$, $n_b$, $n_t$ are numbers of individuals from the focal species
that were sampled for $e$, $b$, and $t$, respectively.
Uppercase letters are used to distinguish inversed parameters.
To estimate the standard error of $a$ ($s_{\bar{a}}$), we did the following:


\begin{equation}
\label{eq:absorption4}
\begin{split}
    s_e^2 &= \frac{1}{n_e-1} \sum_{i=1}^{n_e}\left( e_{i} - \bar{e} \right)^2 \\
    s_B^2 &= \frac{1}{n_b-1} \sum_{i=1}^{n_b}\left( B_{i} - \bar{B} \right)^2 \\
    s_T^2 &= \frac{1}{n_t-1} \sum_{i=1}^{n_t}\left( T_{i} - \bar{T} \right)^2 \\
    s_{eB}^2 &= \left(\bar{e}\right)^2 s_B^2 + \left(\bar{B}\right)^2 s_e^2 + 
        s_e^2 s_B^2 \\
    s_{a}^2 &= \left(\bar{eB}\right)^2 s_T^2 + \left(\bar{T}\right)^2 s_{eB}^2 + 
        s_{eB}^2 s_T^2 \\
    s_{\bar{a}} &= \sqrt{\frac{ s_{a}^2 }{ \min\left( n_e, n_b, n_t \right) }}
\end{split}
\end{equation}


Lastly, we log-transformed $\bar{a}$ and $s_{\bar{a}}$ by using the following:

If\ldots

- $X$ is lognormally distributed with mean $M$ and variance $V$
- $Y = \log\left(X\right)$ with mean $m$ and variance $v$

then\ldots

\begin{equation}
\label{eq:absorption-log}
\begin{split}
    v &= \log\left(\frac{V}{M^2} + 1 \right) \\
    m &= \log\left(M \right) - \frac{v}{2}
\end{split}
\end{equation}

